theories/Semantics.v
@@ -14,7 +14,7 @@ Module Semantics.
     with Value : Type :=
     | V_Nat : nat -> Value
     | V_Bool : bool -> Value
-    | V_Closure : FExpr -> Env -> Value
+    | V_Closure : FExpr_Sub -> Env -> Value
     | V_ReturnValue : Value -> Value.
 
   Fixpoint lookup_env (varName : string) (env : Env) {struct env} : sum string Value :=
@@ -42,7 +42,7 @@ Module Semantics.
 
   Notation "f <*> s" := (sum_ap f s) (at level 50, left associativity).
 
-  Fixpoint Feval (expr : FExpr) (env : Env) (max : nat) : sum (list string) Value :=
+  Fixpoint Feval_Sub (expr : FExpr_Sub) (env : Env) (max : nat) : sum (list string) Value :=
     match max with
     | 0 =>
         inl ("Error: Maximum recursion depth exceeded" :: nil)
@@ -54,45 +54,35 @@ Module Semantics.
               inr value
           | inl err =>
               inl
-                ("(Feval) Error: Unbound variable" :: err :: nil)
+                ("(Feval_Sub) Error: Unbound variable" :: err :: nil)
           end
       | F_Lambda paramName bodyExpr =>
           inr (V_Closure (F_Lambda paramName bodyExpr) env)
       | F_Apply funcExpr argExpr =>
-          match Feval funcExpr env max' with
-          | inr (V_Closure (F_Lambda paramName bodyExpr) _) =>
-              let argValueSum := Feval (F_Return argExpr) env max' in
+          match Feval_Sub funcExpr env max' with
+          | inr (V_Closure (F_Lambda paramName bodyExpr) rest_env) =>
+              let argValueSum := Feval_Sub argExpr rest_env max' in
               match argValueSum with
               | inr argValue =>
-                let extendedEnv := ExtendEnv paramName argValue env in
-                Feval bodyExpr extendedEnv max'
+                let extendedEnv := ExtendEnv paramName argValue rest_env in
+                Feval_Sub bodyExpr extendedEnv max'
               | inl err =>
                   inl
-                    ("(Feval) Error: Function argument did not evaluate to a value"
+                    ("(Feval_Sub) Error: Function argument did not evaluate to a value"
                       :: err)
               end
           | _ =>
               inl
-                ("(Feval) Error: Attempted to apply a non-function" :: nil)
+                ("(Feval_Sub) Error: Attempted to apply a non-function" :: nil)
           end
       | F_Cond condExpr trueExpr falseExpr =>
           match Beval condExpr env max' with
           | inr b =>
               if b
-              then Feval trueExpr env max'
-              else Feval falseExpr env max'
+              then Feval_Sub trueExpr env max'
+              else Feval_Sub falseExpr env max'
           | inl err =>
-              inl ("(Feval) Error: Condition did not evaluate to a boolean" :: err :: nil)
-          end
-      | F_Let varName bindExpr bodyExpr =>
-          let bindValueSum := Feval bindExpr env max' in
-          match bindValueSum with
-          | inr bindValue =>
-            let extendedEnv := ExtendEnv varName bindValue env in
-            Feval bodyExpr extendedEnv max'
-          | inl err =>
-              inl
-                ("(Feval) Error: Let binding did not evaluate to a value" :: err)
+              inl ("(Feval_Sub) Error: Condition did not evaluate to a boolean" :: err :: nil)
           end
       | F_Return retExpr =>
           match retExpr with
@@ -102,7 +92,7 @@ Module Semantics.
                   inr v
               | inl err =>
                   inl
-                    ("(Feval) Error: Boolean expression did not evaluate to a boolean" :: err :: nil)
+                    ("(Feval_Sub) Error: Boolean expression did not evaluate to a boolean" :: err :: nil)
               end
           | E_Arith a =>
               match V_Nat <$> (Aeval a env max') with
@@ -110,7 +100,7 @@ Module Semantics.
                   inr v
               | inl err =>
                   inl
-                    (("(Feval) Error: Arithmetic expression did not evaluate to a number" :: err :: nil))
+                    (("(Feval_Sub) Error: Arithmetic expression did not evaluate to a number" :: err :: nil))
               end
           end
       end
@@ -128,15 +118,23 @@ Module Semantics.
           add <$> (Aeval a1 env max') <*> (Aeval a2 env max')
       | A_Sub a1 a2 =>
           minus <$> (Aeval a1 env max') <*> (Aeval a2 env max')
-      | A_Mult a1 a2 =>
+      | A_Mul a1 a2 =>
           mult <$> (Aeval a1 env max') <*> (Aeval a2 env max')
       | A_Func f =>
-          match Feval f env max' with
+          match Feval_Sub f env max' with
           | inr (V_Nat n) =>
               inr n
           | _ =>
               inl
                 "(Aeval) Error: Function did not evaluate to a number"
+          end
+      | A_Var varName =>
+          match lookup_env varName env with
+          | inr (V_Nat n) =>
+              inr n
+          | _ =>
+              inl
+                "(Aeval) Error: Variable did not evaluate to a number"
           end
       end
     end
@@ -149,10 +147,6 @@ Module Semantics.
       match b with
       | B_Const b =>
           inr b
-      | B_Not b' =>
-          negb <$> Beval b' env max'
-      | B_And b1 b2 =>
-          andb <$> (Beval b1 env max') <*> (Beval b2 env max')
       | B_Eq e1 e2 =>
           match e1, e2 with
           | E_Bool b1, E_Bool b2 =>
@@ -163,17 +157,60 @@ Module Semantics.
               inl
                 ("(Beval) Error: Attempted to compare a boolean to a number")
           end
-      | B_Le b1 b2 =>
-          Nat.leb <$> (Aeval b1 env max') <*> (Aeval b2 env max')
       | B_Func f =>
-          match Feval f env max' with
+          match Feval_Sub f env max' with
           | inr (V_Bool b) =>
               inr b
           | _ =>
               inl
                ("(Beval) Error: Function did not evaluate to a boolean")
           end
+      | B_Var varName =>
+          match lookup_env varName env with
+          | inr (V_Bool b) =>
+              inr b
+          | _ =>
+              inl
+                ("(Beval) Error: Variable did not evaluate to a boolean")
+          end
       end
     end.
+
+  Definition Feval (expr : FExpr) (env : Env) (max : nat) : sum (list string) Value :=
+    match expr with
+    | F_Let varName bindExpr bodyExpr =>
+        let bindValueSum := Feval_Sub bindExpr env max in
+        match bindValueSum with
+        | inr bindValue =>
+          let extendedEnv := ExtendEnv varName bindValue env in
+          Feval_Sub bodyExpr extendedEnv max
+        | inl err =>
+            inl
+              ("(Feval_Sub) Error: Let binding did not evaluate to a value" :: err)
+        end
+    end.
+
+  Compute Feval_Sub ((F_Return (E_Arith (A_Add (A_Const 1) (A_Const 2))))) EmptyEnv 100.
+  Compute Feval (F_Let "x" ((F_Return (E_Arith (A_Add (A_Const 1) (A_Const 2))))) ((F_Return (E_Arith (A_Add (A_Const 3) (A_Func (F_Var "x"))))))) EmptyEnv 100.
+  Compute Feval
+    (F_Let "double"
+      (F_Lambda "n"
+        (F_Return
+          (E_Arith
+            (A_Mul (A_Func (F_Var "n")) (A_Const 2))
+          )
+        )
+      )
+      (F_Apply
+        (F_Var "double")
+        (F_Return
+          (E_Arith
+            (A_Add (A_Const 8) (A_Const 9))
+          )
+        )
+      )
+    )
+    EmptyEnv
+    100.
 
 End Semantics.
