theories/Syntax.v
@@ -3,11 +3,14 @@ From Coq Require Import Strings.String.
 Module Syntax.
 
   Inductive FExpr : Type :=
-  | F_Var : string -> FExpr
-  | F_Lambda : string -> FExpr -> FExpr
-  | F_Apply : FExpr -> Expr -> FExpr
-  | F_Cond : BExpr -> FExpr -> FExpr -> FExpr
-  | F_Return : Expr -> FExpr
+    | F_Let : string -> FExpr_Sub -> FExpr_Sub -> FExpr
+
+  with FExpr_Sub : Type :=
+    | F_Var : string -> FExpr_Sub
+    | F_Lambda : string -> FExpr_Sub -> FExpr_Sub
+    | F_Apply : FExpr_Sub -> FExpr_Sub -> FExpr_Sub
+    | F_Cond : BExpr -> FExpr_Sub -> FExpr_Sub -> FExpr_Sub
+    | F_Return : Expr -> FExpr_Sub
 
   with Expr : Type :=
     | E_Bool : BExpr -> Expr
@@ -16,12 +19,15 @@ Module Syntax.
   with BExpr : Type :=
     | B_Const : bool -> BExpr
     | B_Eq : Expr -> Expr -> BExpr
-    | B_Func : FExpr -> BExpr
+    | B_Func : FExpr_Sub -> BExpr
+    | B_Var : string -> BExpr
 
   with AExpr : Type :=
     | A_Const : nat -> AExpr
     | A_Add : AExpr -> AExpr -> AExpr
     | A_Sub : AExpr -> AExpr -> AExpr
-    | A_Func : FExpr -> AExpr.
+    | A_Mul : AExpr -> AExpr -> AExpr
+    | A_Func : FExpr_Sub -> AExpr
+    | A_Var : string -> AExpr.
 
 End Syntax.
